Rewrite.

theories/data_human_lang/syntax.v
@@ -8,6 +8,13 @@ From camlcert.data_lang Require Export
 From camlcert Require Import
   options.
 
+Implicit Types b : bool.
+Implicit Types n : Z.
+Implicit Types idx : data_index.
+Implicit Types tag : data_tag.
+Implicit Types func : data_function.
+Implicit Types annot : data_annotation.
+
 Notation data_human_name :=
   string
 ( only parsing
@@ -15,11 +22,12 @@ Notation data_human_name :=
 
 Inductive data_human_val :=
   | DataHumanUnit
-  | DataHumanIndex (idx : data_index)
-  | DataHumanTag (tag : data_tag)
-  | DataHumanInt (n : Z)
-  | DataHumanBool (b : bool)
-  | DataHumanFunc (func : data_function) (annot : data_annotation).
+  | DataHumanIndex idx
+  | DataHumanTag tag
+  | DataHumanBool b
+  | DataHumanInt n
+  | DataHumanFunc func annot.
+Implicit Types v : data_human_val.
 
 #[global] Instance data_human_val_inhabited : Inhabited data_human_val :=
   populate DataHumanUnit.
@@ -36,25 +44,25 @@ Proof.
         inr $ inl idx
     | DataHumanTag tag =>
         inr $ inr $ inl tag
-    | DataHumanInt n =>
-        inr $ inr $ inr $ inl n
     | DataHumanBool b =>
-        inr $ inr $ inr $ inr $ inl b
+        inr $ inr $ inr $ inl b
+    | DataHumanInt n =>
+        inr $ inr $ inr $ inr $ inl n
     | DataHumanFunc func annot =>
         inr $ inr $ inr $ inr $ inr (func, annot)
     end.
-  pose decode v :=
-    match v with
+  pose decode _v :=
+    match _v with
     | inl () =>
         DataHumanUnit
     | inr (inl idx) =>
         DataHumanIndex idx
     | inr (inr (inl tag)) =>
         DataHumanTag tag
-    | inr (inr (inr (inl n))) =>
-        DataHumanInt n
-    | inr (inr (inr (inr (inl b)))) =>
+    | inr (inr (inr (inl b))) =>
         DataHumanBool b
+    | inr (inr (inr (inr (inl n)))) =>
+        DataHumanInt n
     | inr (inr (inr (inr (inr (func, annot))))) =>
         DataHumanFunc func annot
     end.
@@ -62,14 +70,14 @@ Proof.
 Qed.
 
 Inductive data_human_expr :=
-  | DataHumanVal (v : data_human_val)
+  | DataHumanVal v
   | DataHumanVar (x : data_human_name)
   | DataHumanLet (x : binder) (e1 e2 : data_human_expr)
   | DataHumanCall (e1 e2 : data_human_expr)
   | DataHumanUnop (op : data_unop) (e : data_human_expr)
   | DataHumanBinop (op : data_binop) (e1 e2 : data_human_expr)
   | DataHumanIf (e0 e1 e2 : data_human_expr)
-  | DataHumanBlock (tag : data_tag) (e1 e2 : data_human_expr)
+  | DataHumanBlock tag (e1 e2 : data_human_expr)
   | DataHumanLoad (e1 e2 : data_human_expr)
   | DataHumanStore (e1 e2 e3 : data_human_expr).
 
@@ -77,58 +85,114 @@ Inductive data_human_expr :=
   populate (DataHumanVal inhabitant).
 #[global] Instance data_human_expr_eq_dec : EqDecision data_human_expr :=
   ltac:(solve_decision).
+Variant data_human_encode_leaf :=
+  | DataHumanEncodeVal v
+  | DataHumanEncodeVar (x : binder)
+  | DataHumanEncodeUnop (op : data_unop)
+  | DataHumanEncodeBinop (op : data_binop)
+  | DataHumanEncodeTag tag.
+#[local] Instance data_human_encode_leaf_eq_dec : EqDecision data_human_encode_leaf :=
+  ltac:(solve_decision).
+#[local] Instance data_human_encode_leaf_countable :
+  Countable data_human_encode_leaf.
+Proof.
+  pose encode leaf :=
+    match leaf with
+    | DataHumanEncodeVal v =>
+        inl $ inl $ inl $ inl v
+    | DataHumanEncodeVar x =>
+        inl $ inl $ inl $ inr x
+    | DataHumanEncodeUnop op =>
+        inl $ inl $ inr op
+    | DataHumanEncodeBinop op =>
+        inl $ inr op
+    | DataHumanEncodeTag tag =>
+        inr tag
+    end.
+  pose decode leaf :=
+    match leaf with
+    | inl (inl (inl (inl v))) =>
+        DataHumanEncodeVal v
+    | inl (inl (inl (inr x))) =>
+        DataHumanEncodeVar x
+    | inl (inl (inr op)) =>
+        DataHumanEncodeUnop op
+    | inl (inr op) =>
+        DataHumanEncodeBinop op
+    | inr tag =>
+        DataHumanEncodeTag tag
+    end.
+  refine (inj_countable' encode decode _). intros []; done.
+Qed.
 #[global] Instance data_human_expr_countable :
   Countable data_human_expr.
 Proof.
+  #[local] Notation code_Let :=
+    0.
+  #[local] Notation code_Call :=
+    1.
+  #[local] Notation code_Unop :=
+    2.
+  #[local] Notation code_Binop :=
+    3.
+  #[local] Notation code_If :=
+    4.
+  #[local] Notation code_Block :=
+    5.
+  #[local] Notation code_Load :=
+    6.
+  #[local] Notation code_Store :=
+    7.
   pose fix encode e :=
     match e with
     | DataHumanVal v =>
-        GenLeaf (inl v)
+        GenLeaf (DataHumanEncodeVal v)
     | DataHumanVar x =>
-        GenLeaf (inr $ inl $ BNamed x)
+        GenLeaf (DataHumanEncodeVar (BNamed x))
     | DataHumanLet x e1 e2 =>
-        GenNode 0 [GenLeaf (inr $ inl x); encode e1; encode e2]
+        GenNode code_Let [GenLeaf (DataHumanEncodeVar x); encode e1; encode e2]
     | DataHumanCall e1 e2 =>
-        GenNode 1 [encode e1; encode e2]
+        GenNode code_Call [encode e1; encode e2]
     | DataHumanUnop op e =>
-        GenNode 2 [GenLeaf (inr $ inr $ inl op); encode e]
+        GenNode code_Unop [GenLeaf (DataHumanEncodeUnop op); encode e]
     | DataHumanBinop op e1 e2 =>
-        GenNode 3 [GenLeaf (inr $ inr $ inr $ inl op); encode e1; encode e2]
+        GenNode code_Binop [GenLeaf (DataHumanEncodeBinop op); encode e1; encode e2]
     | DataHumanIf e0 e1 e2 =>
-        GenNode 4 [encode e0; encode e1; encode e2]
+        GenNode code_If [encode e0; encode e1; encode e2]
     | DataHumanBlock tag e1 e2 =>
-        GenNode 5 [GenLeaf (inr $ inr $ inr $ inr tag); encode e1; encode e2]
+        GenNode code_Block [GenLeaf (DataHumanEncodeTag tag); encode e1; encode e2]
     | DataHumanLoad e1 e2 =>
-        GenNode 6 [encode e1; encode e2]
+        GenNode code_Load [encode e1; encode e2]
     | DataHumanStore e1 e2 e3 =>
-        GenNode 7 [encode e1; encode e2; encode e3]
+        GenNode code_Store [encode e1; encode e2; encode e3]
     end.
-  pose fix decode e :=
-    match e with
-    | GenLeaf (inl v) =>
+  pose fix decode _e :=
+    match _e with
+    | GenLeaf (DataHumanEncodeVal v) =>
         DataHumanVal v
-    | GenLeaf (inr (inl (BNamed x))) =>
+    | GenLeaf (DataHumanEncodeVar (BNamed x)) =>
         DataHumanVar x
-    | GenNode 0 [GenLeaf (inr (inl x)); e1; e2] =>
+    | GenNode code_Let [GenLeaf (DataHumanEncodeVar x); e1; e2] =>
         DataHumanLet x (decode e1) (decode e2)
-    | GenNode 1 [e1; e2] =>
+    | GenNode code_Call [e1; e2] =>
         DataHumanCall (decode e1) (decode e2)
-    | GenNode 2 [GenLeaf (inr (inr (inl op))); e] =>
+    | GenNode code_Unop [GenLeaf (DataHumanEncodeUnop op); e] =>
         DataHumanUnop op (decode e)
-    | GenNode 3 [GenLeaf (inr (inr (inr (inl op)))); e1; e2] =>
+    | GenNode code_Binop [GenLeaf (DataHumanEncodeBinop op); e1; e2] =>
         DataHumanBinop op (decode e1) (decode e2)
-    | GenNode 4 [e0; e1; e2] =>
+    | GenNode code_If [e0; e1; e2] =>
         DataHumanIf (decode e0) (decode e1) (decode e2)
-    | GenNode 5 [GenLeaf (inr (inr (inr (inr tag)))); e1; e2] =>
+    | GenNode code_Block [GenLeaf (DataHumanEncodeTag tag); e1; e2] =>
         DataHumanBlock tag (decode e1) (decode e2)
-    | GenNode 6 [e1; e2] =>
+    | GenNode code_Load [e1; e2] =>
         DataHumanLoad (decode e1) (decode e2)
-    | GenNode 7 [e1; e2; e3] =>
+    | GenNode code_Store [e1; e2; e3] =>
         DataHumanStore (decode e1) (decode e2) (decode e3)
     | _ =>
         @inhabitant _ data_human_expr_inhabited
     end.
-  apply (inj_countable' encode decode). intros e. induction e; simpl; congruence.
+  apply (inj_countable' encode decode).
+  intros e. induction e; simpl; congruence.
 Qed.
 
 Record data_human_definition := {
