theories/data_lang/language.v
@@ -7,67 +7,12 @@ From camlcert.data_lang Require Export
 From camlcert Require Import
   options.
 
-Implicit Types l : loc.
-Implicit Types v w : data_val.
-Implicit Types e : data_expr.
-Implicit Types σ : data_state.
-
-Notation data_of_val :=
-  DataVal.
-
-Definition data_to_val e :=
-  match e with
-  | DataVal v => Some v
-  | _ => None
-  end.
-
 Canonical data_val_O :=
   leibnizO data_val.
 Canonical data_expr_O :=
   leibnizO data_expr.
 Canonical data_state_O :=
   leibnizO data_state.
-
-Inductive data_ectxi :=
-  | DataEctxiLet e2
-  | DataEctxiCall1 e1
-  | DataEctxiCall2 v2
-  | DataEctxiUnop (op : data_unop)
-  | DataEctxiIf e1 e2
-  | DataEctxiLoad1 e1
-  | DataEctxiLoad2 v2
-  | DataEctxiStore1 e1 e2
-  | DataEctxiStore2 e1 v3
-  | DataEctxiStore3 v2 v3.
-
-Definition data_ectx :=
-  list data_ectxi.
-
-Definition data_fill_item k e :=
-  match k with
-  | DataEctxiLet e2 =>
-      DataLet e e2
-  | DataEctxiCall1 e1 =>
-      DataCall e1 e
-  | DataEctxiCall2 v2 =>
-      DataCall e (data_of_val v2)
-  | DataEctxiUnop op =>
-      DataUnop op e
-  | DataEctxiIf e1 e2 =>
-      DataIf e e1 e2
-  | DataEctxiLoad1 e1 =>
-      DataLoad e1 e
-  | DataEctxiLoad2 v2 =>
-      DataLoad e (data_of_val v2)
-  | DataEctxiStore1 e1 e2 =>
-      DataStore e1 e2 e
-  | DataEctxiStore2 e1 v3 =>
-      DataStore e1 e (data_of_val v3)
-  | DataEctxiStore3 v2 v3 =>
-      DataStore e (data_of_val v2) (data_of_val v3)
-  end.
-#[global] Instance data_ectxi_fill : Fill data_ectxi data_expr :=
-  Build_Fill data_fill_item.
 
 Lemma data_ectxi_lang_mixin :
   EctxiLanguageMixin
@@ -77,13 +22,13 @@ Lemma data_ectxi_lang_mixin :
     data_ectxi.
 Proof.
   split.
-  - naive_solver.
-  - intros []; naive_solver.
-  - intros * []; naive_solver.
-  - intros [] ?**; naive_solver.
-  - intros []; naive_solver.
-  - intros [] ? []; naive_solver.
-  - intros ? [] * Hstep; invert Hstep; naive_solver.
+  - apply data_to_of_val.
+  - apply data_of_to_val.
+  - apply data_head_step_not_val.
+  - apply _.
+  - apply data_ectxi_fill_not_val .
+  - apply data_ectxi_fill_no_val_inj.
+  - apply data_ectxi_fill_head_step_val.
 Qed.
 Canonical data_ectxi_lang :=
   Build_ectxi_language data_ectxi_lang_mixin.
