theories/data_lang/semantics.v
@@ -2,13 +2,22 @@ From camlcert Require Import
   prelude.
 From camlcert.data_lang Require Export
   syntax.
-From camlcert.data_lang Require Import
-  notations.
 From camlcert Require Import
   options.
 
+Implicit Types b : bool.
+Implicit Types l : loc.
+Implicit Types func : data_function.
+Implicit Types annot : data_annotation.
+Implicit Types tag : data_tag.
+Implicit Types idx : data_index.
+Implicit Types v w : data_val.
+Implicit Types e : data_expr.
+Implicit Types prog : data_program.
+
 Definition data_state :=
   gmap loc data_val.
+Implicit Types σ : data_state.
 
 #[global] Instance data_state_eq_dec :
   EqDecision data_state.
@@ -20,17 +29,6 @@ Defined.
 Proof.
   apply _.
 Qed.
-
-Implicit Types b : bool.
-Implicit Types l : loc.
-Implicit Types func : data_function.
-Implicit Types annot : data_annotation.
-Implicit Types tag : data_tag.
-Implicit Types idx : data_index.
-Implicit Types v w : data_val.
-Implicit Types e : data_expr.
-Implicit Types prog : data_program.
-Implicit Types σ : data_state.
 
 Definition data_unop_eval op v :=
   match op, v with
@@ -86,78 +84,185 @@ Definition data_binop_eval op v1 v2 :=
 
 Inductive data_head_step prog : data_expr → data_state → data_expr → data_state → Prop :=
   | data_head_step_let v e e' σ :
-      e' = e.[#v/] →
+      e' = e.[DataVal v/] →
       data_head_step prog
-        (let: v in e) σ
-        e' σ
+        (DataLet (DataVal v) e)
+        σ
+        e'
+        σ
   | data_head_step_call func def annot v e e' σ :
       prog !! func = Some def →
       e = def.(data_definition_body) →
-      e' = e.[#v/] →
+      e' = e.[DataVal v/] →
       data_head_step prog
-        ((DataFunc func annot) v) σ
-        e' σ
+        (DataCall (DataVal $ DataFunc func annot) (DataVal v))
+        σ
+        e'
+        σ
   | data_head_step_unop op v v' σ :
       data_unop_eval op v = Some v' →
       data_head_step prog
-        (DataUnop op v) σ
-        v' σ
+        (DataUnop op (DataVal v))
+        σ
+        (DataVal v')
+        σ
   | data_head_step_binop_1 op e1 e2 e' σ :
-      e' = (let: e1 in let: e2.[ren (+1)] in DataBinopDet op $1 $0)%data_expr →
+      e' = DataLet e1 $ DataLet e2.[ren (+1)] $ DataBinopDet op (DataVar 1) (DataVar 0) →
       data_head_step prog
-        (DataBinop op e1 e2) σ
-        e' σ
+        (DataBinop op e1 e2)
+        σ
+        e'
+        σ
   | data_head_step_binop_2 op e1 e2 e' σ :
-      e' = (let: e2 in let: e1.[ren (+1)] in DataBinopDet op $0 $1)%data_expr →
+      e' = DataLet e2 $ DataLet e1.[ren (+1)] $ DataBinopDet op (DataVar 0) (DataVar 1) →
       data_head_step prog
-        (DataBinop op e1 e2) σ
-        e' σ
+        (DataBinop op e1 e2)
+        σ
+        e'
+        σ
   | data_head_step_binop_det op v1 v2 v' σ :
       data_binop_eval op v1 v2 = Some v' →
       data_head_step prog
-        (DataBinopDet op v1 v2) σ
-        v' σ
+        (DataBinopDet op (DataVal v1) (DataVal v2))
+        σ
+        (DataVal v')
+        σ
   | data_head_step_if b e1 e2 σ :
       data_head_step prog
-        (if: b then e1 else e2) σ
-        (if b then e1 else e2) σ
+        (DataIf (DataVal $ DataBool b) e1 e2)
+        σ
+        (if b then e1 else e2)
+        σ
   | data_head_step_block_1 tag e1 e2 e' σ :
-      e' = (let: e1 in let: e2.[ren (+1)] in &&tag $1 $0)%data_expr →
+      e' = DataLet e1 $ DataLet e2.[ren (+1)] $ DataBlockDet tag (DataVar 1) (DataVar 0) →
       data_head_step prog
-        (&tag e1 e2) σ
-        e' σ
+        (DataBlock tag e1 e2)
+        σ
+        e'
+        σ
   | data_head_step_block_2 tag e1 e2 e' σ :
-      e' = (let: e2 in let: e1.[ren (+1)] in &&tag $0 $1)%data_expr →
+      e' = DataLet e2 $ DataLet e1.[ren (+1)] $ DataBlockDet tag (DataVar 0) (DataVar 1) →
       data_head_step prog
-        (&tag e1 e2) σ
-        e' σ
+        (DataBlock tag e1 e2)
+        σ
+        e'
+        σ
   | data_head_step_block_det tag v1 v2 σ l :
       σ !! (l +ₗ 0) = None →
       σ !! (l +ₗ 1) = None →
       σ !! (l +ₗ 2) = None →
       data_head_step prog
-        (&&tag v1 v2) σ
-        l (<[l +ₗ 2 := v2]> (<[l +ₗ 1 := v1]> (<[l +ₗ 0 := DataTag tag]> σ)))
+        (DataBlockDet tag (DataVal v1) (DataVal v2))
+        σ
+        (DataVal $ DataLoc l)
+        (<[l +ₗ 2 := v2]> (<[l +ₗ 1 := v1]> (<[l +ₗ 0 := DataTag tag]> σ)))
   | data_head_step_load l l' idx v σ :
       σ !! (l +ₗ idx) = Some v →
       data_head_step prog
-        (![idx] l) σ
-        v σ
+        (DataLoad (DataVal $ DataLoc l) (DataVal $ DataIndex idx))
+        σ
+        (DataVal v)
+        σ
   | data_head_step_store l idx v w σ :
       σ !! (l +ₗ idx) = Some v →
       data_head_step prog
-        (l <-[idx] w) σ
-        #() (<[l +ₗ idx := w]> σ).
+        (DataStore (DataVal $ DataLoc l) (DataVal $ DataIndex idx) (DataVal w))
+        σ
+        (DataVal DataUnit)
+        (<[l +ₗ idx := w]> σ).
 
 Lemma data_head_step_block_det' prog tag v1 v2 σ σ' :
   let l := loc_fresh (dom σ) in
   σ' = <[l +ₗ 2 := v2]> (<[l +ₗ 1 := v1]> (<[l +ₗ 0 := DataTag tag]> σ)) →
   data_head_step prog
-    (&&tag v1 v2) σ
-    l σ'.
+    (DataBlockDet tag (DataVal v1) (DataVal v2))
+    σ
+    (DataVal $ DataLoc l)
+    σ'.
 Proof.
   intros l ->.
   apply data_head_step_block_det;
     rewrite -not_elem_of_dom;
     apply loc_fresh_fresh; lia.
 Qed.
+
+Lemma data_head_step_not_val prog e1 σ1 e2 σ2 :
+  data_head_step prog e1 σ1 e2 σ2 →
+  data_to_val e1 = None.
+Proof.
+  destruct 1; naive_solver.
+Qed.
+
+Inductive data_ectxi :=
+  | DataEctxiLet e2
+  | DataEctxiCall1 e1
+  | DataEctxiCall2 v2
+  | DataEctxiUnop (op : data_unop)
+  | DataEctxiIf e1 e2
+  | DataEctxiLoad1 e1
+  | DataEctxiLoad2 v2
+  | DataEctxiStore1 e1 e2
+  | DataEctxiStore2 e1 v3
+  | DataEctxiStore3 v2 v3.
+
+Definition data_ectxi_fill k e :=
+  match k with
+  | DataEctxiLet e2 =>
+      DataLet e e2
+  | DataEctxiCall1 e1 =>
+      DataCall e1 e
+  | DataEctxiCall2 v2 =>
+      DataCall e (DataVal v2)
+  | DataEctxiUnop op =>
+      DataUnop op e
+  | DataEctxiIf e1 e2 =>
+      DataIf e e1 e2
+  | DataEctxiLoad1 e1 =>
+      DataLoad e1 e
+  | DataEctxiLoad2 v2 =>
+      DataLoad e (DataVal v2)
+  | DataEctxiStore1 e1 e2 =>
+      DataStore e1 e2 e
+  | DataEctxiStore2 e1 v3 =>
+      DataStore e1 e (DataVal v3)
+  | DataEctxiStore3 v2 v3 =>
+      DataStore e (DataVal v2) (DataVal v3)
+  end.
+#[global] Arguments data_ectxi_fill !_ _ / : assert.
+#[global] Instance data_ectxi_fill_ : Fill data_ectxi data_expr :=
+  Build_Fill data_ectxi_fill.
+
+#[global] Instance data_ectxi_fill_inj k :
+  Inj (=) (=) (k @@.).
+Proof.
+  induction k; intros ?*; naive_solver.
+Qed.
+Lemma data_ectxi_fill_val k e :
+  is_Some (data_to_val (k @@ e)) →
+  is_Some (data_to_val e).
+Proof.
+  intros (v & ?). destruct k; done.
+Qed.
+Lemma data_ectxi_fill_not_val k e :
+  data_to_val e = None →
+  data_to_val (k @@ e) = None.
+Proof.
+  destruct k; done.
+Qed.
+Lemma data_ectxi_fill_no_val_inj k1 e1 k2 e2 :
+  data_to_val e1 = None →
+  data_to_val e2 = None →
+  k1 @@ e1 = k2 @@ e2 →
+  k1 = k2.
+Proof.
+  destruct k1, k2; naive_solver.
+Qed.
+Lemma data_ectxi_fill_head_step_val prog k e σ1 e2 σ2 :
+  data_head_step prog (k @@ e) σ1 e2 σ2 →
+  is_Some (data_to_val e).
+Proof.
+  destruct k; inversion_clear 1; done.
+Qed.
+
+Definition data_ectx :=
+  list data_ectxi.
